now deployable, with low z3rlimit

Oracle2/Oracle2.fst
@@ -24,7 +24,7 @@ type assets =
 // compressed public key
 type cpk = byte ** hash
 
-let parseArgs (msg: option data): result args `cost` 194 =
+let parseArgs (msg: option data): result args `cost` 235 = // 41
     let open OT in
     match msg with
     | Some (Collection (Dict dict)) -> begin
@@ -45,33 +45,32 @@ let parseArgs (msg: option data): result args `cost` 194 =
     | _ -> RT.autoFailw "MessageBody must be a dictionary."
 
 // compress a public key
-val compress: publicKey -> cpk `cost` 132
-let compress pk = let open FStar.UInt8 in // 13
+let compress (pk:publicKey): cpk `cost` 305 = let open FStar.UInt8 in // 13
     let parity = (Zen.Array.item 32 pk %^ 2uy) +^ 2uy in
-    let aux (i:nat{i < 32}) (* : byte `cost` 5 *) =
+    let aux (i:nat{i < 32}): byte `cost` 5 =
         ret (Zen.Array.item (31-i) pk) in
     let! x = Zen.Array.init_pure 32 aux in // 292
     ret (parity, x)
 
-let updateCPK ((parity, h):cpk) (s:Sha3.t): Sha3.t `cost` 198 =
+let updateCPK ((parity, h):cpk) (s:Sha3.t): Sha3.t `cost` 203 = // 5
     Sha3.updateByte parity Sha3.empty
     >>= Sha3.updateHash h
 
 // hash a compressed publicKey
-let hashCPK (cpk:cpk): hash `cost` 218 =
-    updateCPK cpk Sha3.empty // 198
+let hashCPK (cpk:cpk): hash `cost` 227 = // 4
+    updateCPK cpk Sha3.empty // 203
     >>= Sha3.finalize // 20
 
-let hashArgs (args:args{Some? args.oraclePubKey}): hash `cost` 590 =
-    let! cpk = compress (Some?.v args.oraclePubKey) in // 132
+let hashArgs (args:args{Some? args.oraclePubKey}): hash `cost` 786 = // 18
+    let! cpk = compress (Some?.v args.oraclePubKey) in // 305
     Sha3.updateHash args.commit Sha3.empty // 192
     >>= Sha3.updateU64 args.timestamp // 48
-    >>= updateCPK cpk // 198
+    >>= updateCPK cpk // 203
     >>= Sha3.finalize // 20
 
-val mkAssets: contractId -> args:args{Some? args.oraclePubKey} -> assets `cost` 802
-let mkAssets (v, h) args =
-    let! argsHash = hashArgs args in // 590
+val mkAssets: contractId -> args:args{Some? args.oraclePubKey} -> assets `cost` 1016
+let mkAssets (v, h) args = // 18
+    let! argsHash = hashArgs args in // 786
     let! arsgHash2 = Sha3.updateHash argsHash Sha3.empty // 192
                      >>= Sha3.finalize in // 20
     ret ({ commitment=v,h,argsHash; attestation=v,h,arsgHash2 })
@@ -80,10 +79,10 @@ let mkAssets (v, h) args =
 // Making a commitment
 //
 
-val commit: txSkeleton -> contractId -> publicKey -> args -> CR.t `cost` 933
-let commit tx cid senderPK args =
+val commit: txSkeleton -> contractId -> publicKey -> args -> CR.t `cost` 1163
+let commit tx cid senderPK args = // 16
     let args = { args with oraclePubKey=Some senderPK } in
-    let! ({commitment=commitment}) = mkAssets cid args in // 802
+    let! ({commitment=commitment}) = mkAssets cid args in // 1016
     // mint the commitment token
     TX.mint 1UL commitment tx // 64
     // lock the commitment token to the contract
@@ -95,30 +94,28 @@ let commit tx cid senderPK args =
 // Attesting to a commitment
 //
 
-let lockToPK (s:spend) (pk:publicKey) (tx:txSkeleton): txSkeleton `cost` 414 =
-    let! pkHash = compress pk >>= hashCPK in // 132 + 218
-    TX.lockToAddress s.asset s.amount (PKLock pkHash) tx
+let lockToPK (s:spend) (pk:publicKey) (tx:txSkeleton): txSkeleton `cost` 608 = // 12
+    let! pkHash = compress pk >>= hashCPK in // 305 + 227
+    TX.lockToAddress s.asset s.amount (PKLock pkHash) tx // 64
 
-// the attestation transaction, minus contract wallet inputs
-let attestTx tx cid senderPK assets: txSkeleton `cost` 670 =
+// The attestation transaction, minus contract wallet inputs
+let attestTx tx cid senderPK assets: txSkeleton `cost` 891 = // 27
     // destroy the attestation token
     TX.destroy 1UL assets.commitment tx // 64
     // mint the new commitment and attestation tokens
     >>= TX.mint 1UL assets.commitment // 64
     >>= TX.mint 1UL assets.attestation // 64
     // lock the attestation token to the user
-    >>= lockToPK ({asset=assets.attestation; amount=1UL}) senderPK // 414
+    >>= lockToPK ({asset=assets.attestation; amount=1UL}) senderPK // 608
     // lock the commitment token to the contract
     >>= TX.lockToContract assets.commitment 1UL cid // 64
 
-//val attest: txSkeleton -> contractId -> publicKey -> w:wallet -> args
-//            -> CR.t `cost` (W.size w * 128 + 1539)
-let attest' tx cid senderPK w (args:args) =
+let attest' tx cid senderPK w (args:args) = // 22
     match args.oraclePubKey with
     | Some _ -> begin
-        let! assets = mkAssets cid args in // 802
+        let! assets = mkAssets cid args in // 1016
         // the tx, minus contract wallet inputs
-        attestTx tx cid senderPK assets
+        attestTx tx cid senderPK assets // 891
         // add a commitment token from the contract wallet
         >>= TX.fromWallet assets.commitment 1UL cid w // W.size w * 128 + 192
         // return the tx
@@ -128,44 +125,35 @@ let attest' tx cid senderPK w (args:args) =
         RT.autoFailw "Could not parse OraclePubKey"
 
 let attest: txSkeleton -> contractId -> publicKey -> w:wallet -> args
-            -> CR.t `cost` (W.size w * 128 + 1667) = attest'
-
+            -> CR.t `cost` (W.size w * 128 + 2124) = attest'
 
 //
 // Exports
 //
-val main:
-    txSkeleton
-    -> context
-    -> contractId
-    -> command: string
-    -> sender: sender
-    -> option data
-    -> w: wallet
-    -> option data
-    -> CR.t `cost` ( match command, sender with
-                     | "Commit", PK _ -> 1127
-                     | "Attest", PK _ -> Zen.Wallet.size w * 128 + 1861
-                     | _ -> 0 )
-let main tx _ cid command sender msg w _ =
+
+val main: txSkeleton -> context -> contractId -> command: string
+          -> sender: sender -> option data -> w: wallet -> option data
+          -> CR.t `cost` begin match command, sender with
+                         | "Commit", PK _ -> 1418
+                         | "Attest", PK _ -> Zen.Wallet.size w * 128 + 2379
+                         | _ -> 20 end
+let main tx _ cid command sender msg w _ = // 20
     match command, sender with
     | "Commit", PK pk ->
-        parseArgs msg `RT.bind` commit tx cid pk // 194 + 933
-        <: CR.t `cost` begin
-            match command, sender with
-            | "Commit", PK _ -> 1127
-            | "Attest", PK _ -> Zen.Wallet.size w * 128 + 1861
-            | _ -> 0
-            end
+        parseArgs msg `RT.bind` commit tx cid pk // 235 + 1163
+        <: CR.t `cost` begin match command, sender with
+                       | "Commit", PK _ -> 1398
+                       | "Attest", PK _ -> Zen.Wallet.size w * 128 + 2359
+                       | _ -> 0 end
     | "Attest", PK pk ->
-        parseArgs msg `RT.bind` attest tx cid pk w // 194 + (Zen.Wallet.size w * 128 + 1667)
+        parseArgs msg `RT.bind` attest tx cid pk w // 235 + (Zen.Wallet.size w * 128 + 2124)
     | _, PK pk ->
         RT.failw "a"
     | _, _ ->
         RT.failw "b"
 
-let cf _ _ command sender _ w _ =
-    ret ( match command, sender with
-          | "Commit", PK _ -> 1127
-          | "Attest", PK _ -> Zen.Wallet.size w * 128 + 1861
-          | _ -> 0 )
+let cf _ _ command sender _ w _ : nat `cost` 15 = // 15
+    ret begin match command, sender with
+        | "Commit", PK _ -> 1418
+        | "Attest", PK _ -> Zen.Wallet.size w * 128 + 2379
+        | _ -> 20 end
